Rename weak-classical-logic into DeMorgan-logic.

PropositionalLogic/ProofTheory/DeMorgan.v
@@ -11,11 +11,11 @@ Local Open Scope logic_base.
 Local Open Scope syntax.
 Import PropositionalLanguageNotation.
 
-Class WeakClassicalPropositionalLogic (L: Language) {nL: NormalLanguage L} {pL: PropositionalLanguage L} (Gamma: ProofTheory L) {nGamma: NormalProofTheory L Gamma} {mpGamma: MinimunPropositionalLogic L Gamma} {ipGamma: IntuitionisticPropositionalLogic L Gamma} := {
+Class DeMorganPropositionalLogic (L: Language) {nL: NormalLanguage L} {pL: PropositionalLanguage L} (Gamma: ProofTheory L) {nGamma: NormalProofTheory L Gamma} {mpGamma: MinimunPropositionalLogic L Gamma} {ipGamma: IntuitionisticPropositionalLogic L Gamma} := {
   weak_excluded_middle: forall x, |-- ~~ x || ~~ ~~ x
 }.
 
-Lemma derivable_weak_excluded_middle: forall {L: Language} {nL: NormalLanguage L} {pL: PropositionalLanguage L} {Gamma: ProofTheory L} {nGamma: NormalProofTheory L Gamma} {mpGamma: MinimunPropositionalLogic L Gamma} {ipGamma: IntuitionisticPropositionalLogic L Gamma} {wcpGamma: WeakClassicalPropositionalLogic L Gamma} (Phi: context) (x: expr),
+Lemma derivable_weak_excluded_middle: forall {L: Language} {nL: NormalLanguage L} {pL: PropositionalLanguage L} {Gamma: ProofTheory L} {nGamma: NormalProofTheory L Gamma} {mpGamma: MinimunPropositionalLogic L Gamma} {ipGamma: IntuitionisticPropositionalLogic L Gamma} {dmpGamma: DeMorganPropositionalLogic L Gamma} (Phi: context) (x: expr),
   Phi |-- ~~ x || ~~ ~~ x.
 Proof.
   intros.
@@ -23,7 +23,7 @@ Proof.
   apply deduction_weaken0; auto.
 Qed.
 
-Lemma demorgan_negp_andp: forall {L: Language} {nL: NormalLanguage L} {pL: PropositionalLanguage L} {Gamma: ProofTheory L} {nGamma: NormalProofTheory L Gamma} {mpGamma: MinimunPropositionalLogic L Gamma} {ipGamma: IntuitionisticPropositionalLogic L Gamma} {wcpGamma: WeakClassicalPropositionalLogic L Gamma} (x y: expr),
+Lemma demorgan_negp_andp: forall {L: Language} {nL: NormalLanguage L} {pL: PropositionalLanguage L} {Gamma: ProofTheory L} {nGamma: NormalProofTheory L Gamma} {mpGamma: MinimunPropositionalLogic L Gamma} {ipGamma: IntuitionisticPropositionalLogic L Gamma} {dmpGamma: DeMorganPropositionalLogic L Gamma} (x y: expr),
   |-- ~~ (x && y) <--> (~~ x || ~~ y).
 Proof.
   intros.
