SeparationLogic/ProofTheory/IterSepcon.v
@@ -13,7 +13,7 @@ Require Import Logic.MinimunLogic.ProofTheory.Minimun.
 Require Import Logic.MinimunLogic.ProofTheory.RewriteClass.
 Require Import Logic.MinimunLogic.ProofTheory.ContextProperty.
 Require Import Logic.PropositionalLogic.ProofTheory.Intuitionistic.
-Require Import Logic.PropositionalLogic.ProofTheory.WeakClassical.
+Require Import Logic.PropositionalLogic.ProofTheory.DeMorgan.
 Require Import Logic.PropositionalLogic.ProofTheory.GodelDummett.
 Require Import Logic.PropositionalLogic.ProofTheory.Classical.
 Require Import Logic.PropositionalLogic.ProofTheory.RewriteClass.
